Stateful SHA2_512: passing all test vectors

code/experimental/hash/Hacl.Test.SHA2_512.fst
@@ -3,7 +3,7 @@ module Hacl.Test.SHA2_512
 open FStar.Buffer
 open FStar.UInt32
 
-module SHA = SHA2_512
+module Hash = SHA2_512
 
 
 val test_1a: unit -> ST unit
@@ -34,12 +34,12 @@ let test_1a () =
     ] in
 
   (* Allocate memory for state *)
-  let ctx = FStar.Buffer.create 0uL SHA.hash_size_state_512 in
+  let state = FStar.Buffer.create 0uL Hash.size_state in
 
   (* Call the hash function *)
-  SHA.sha2_init_512 ctx;
-  SHA.sha2_update_last_512 ctx plaintext plaintext_len;
-  SHA.sha2_finish_512 ctx output;
+  Hash.init state;
+  Hash.update_last state plaintext (FStar.Int.Cast.uint32_to_uint64 plaintext_len);
+  Hash.finish state output;
 
   (* Display the result *)
   TestLib.compare_and_print (C.string_of_literal "Test 1a") expected output 64ul;
@@ -76,10 +76,10 @@ let test_1b () =
     ] in
 
   (* Allocate memory for state *)
-  let ctx = FStar.Buffer.create 0uL SHA.hash_size_state_512 in
+  let state = FStar.Buffer.create 0uL Hash.size_state in
 
   (* Call the hash function *)
-  SHA.sha2_512 output plaintext plaintext_len;
+  Hash.hash output plaintext plaintext_len;
 
   (* Display the result *)
   TestLib.compare_and_print (C.string_of_literal "Test 1b") expected output 64ul;
@@ -89,74 +89,82 @@ let test_1b () =
 
 
 
-(* val test_2a: unit -> ST unit *)
-(*   (requires (fun h -> True)) *)
-(*   (ensures  (fun h0 r h1 -> True)) *)
-(* let test_2a () = *)
+val test_2a: unit -> ST unit
+  (requires (fun h -> True))
+  (ensures  (fun h0 r h1 -> True))
+let test_2a () =
 
-(*   (\* Push a new memory frame *\) *)
-(*   (\**\) push_frame(); *)
+  (* Push a new memory frame *)
+  (**) push_frame();
 
-(*   let output_len = 64ul in *)
-(*   let output = FStar.Buffer.create 0uy output_len in *)
+  let output_len = 64ul in
+  let output = FStar.Buffer.create 0uy output_len in
 
-(*   let plaintext_len = 0ul in *)
-(*   let plaintext = FStar.Buffer.createL [] in *)
+  let plaintext_len = 0ul in
+  let plaintext = FStar.Buffer.createL [] in
 
-(*   let expected = FStar.Buffer.createL [ *)
-(*       0xe3uy; 0xb0uy; 0xc4uy; 0x42uy; 0x98uy; 0xfcuy; 0x1cuy; 0x14uy; *)
-(*       0x9auy; 0xfbuy; 0xf4uy; 0xc8uy; 0x99uy; 0x6fuy; 0xb9uy; 0x24uy; *)
-(*       0x27uy; 0xaeuy; 0x41uy; 0xe4uy; 0x64uy; 0x9buy; 0x93uy; 0x4cuy; *)
-(*       0xa4uy; 0x95uy; 0x99uy; 0x1buy; 0x78uy; 0x52uy; 0xb8uy; 0x55uy *)
-(*     ] in *)
+  let expected = FStar.Buffer.createL [
+    0xcfuy; 0x83uy; 0xe1uy; 0x35uy; 0x7euy; 0xefuy; 0xb8uy; 0xbduy;
+    0xf1uy; 0x54uy; 0x28uy; 0x50uy; 0xd6uy; 0x6duy; 0x80uy; 0x07uy;
+    0xd6uy; 0x20uy; 0xe4uy; 0x05uy; 0x0buy; 0x57uy; 0x15uy; 0xdcuy;
+    0x83uy; 0xf4uy; 0xa9uy; 0x21uy; 0xd3uy; 0x6cuy; 0xe9uy; 0xceuy;
+    0x47uy; 0xd0uy; 0xd1uy; 0x3cuy; 0x5duy; 0x85uy; 0xf2uy; 0xb0uy;
+    0xffuy; 0x83uy; 0x18uy; 0xd2uy; 0x87uy; 0x7euy; 0xecuy; 0x2fuy;
+    0x63uy; 0xb9uy; 0x31uy; 0xbduy; 0x47uy; 0x41uy; 0x7auy; 0x81uy;
+    0xa5uy; 0x38uy; 0x32uy; 0x7auy; 0xf9uy; 0x27uy; 0xdauy; 0x3euy
+    ] in
 
-(*   (\* Allocate memory for state *\) *)
-(*   let ctx = FStar.Buffer.create 0uL SHA.hash_size_state_512 in *)
+  (* Allocate memory for state *)
+  let state = FStar.Buffer.create 0uL Hash.size_state in
 
-(*   (\* Call the hash function *\) *)
-(*   SHA.sha2_init_512 ctx; *)
-(*   SHA.sha2_update_last_512 ctx plaintext plaintext_len; *)
-(*   SHA.sha2_finish_512 ctx output; *)
+  (* Call the hash function *)
+  Hash.init state;
+  Hash.update_last state plaintext (FStar.Int.Cast.uint32_to_uint64 plaintext_len);
+  Hash.finish state output;
 
-(*   (\* Display the result *\) *)
-(*   TestLib.compare_and_print (C.string_of_literal "Test 2a") expected output 64ul; *)
+  (* Display the result *)
+  TestLib.compare_and_print (C.string_of_literal "Test 2a") expected output 64ul;
 
-(*   (\* Pop the memory frame *\) *)
-(*   (\**\) pop_frame() *)
+  (* Pop the memory frame *)
+  (**) pop_frame()
 
 
-(* val test_2b: unit -> ST unit *)
-(*   (requires (fun h -> True)) *)
-(*   (ensures  (fun h0 r h1 -> True)) *)
-(* let test_2b () = *)
+val test_2b: unit -> ST unit
+  (requires (fun h -> True))
+  (ensures  (fun h0 r h1 -> True))
+let test_2b () =
 
-(*   (\* Push a new memory frame *\) *)
-(*   (\**\) push_frame(); *)
+  (* Push a new memory frame *)
+  (**) push_frame();
 
-(*   let output_len = 32ul in *)
-(*   let output = FStar.Buffer.create 0uy output_len in *)
+  let output_len = 64ul in
+  let output = FStar.Buffer.create 0uy output_len in
 
-(*   let plaintext_len = 0ul in *)
-(*   let plaintext = FStar.Buffer.createL [] in *)
+  let plaintext_len = 0ul in
+  let plaintext = FStar.Buffer.createL [] in
 
-(*   let expected = FStar.Buffer.createL [ *)
-(*       0xe3uy; 0xb0uy; 0xc4uy; 0x42uy; 0x98uy; 0xfcuy; 0x1cuy; 0x14uy; *)
-(*       0x9auy; 0xfbuy; 0xf4uy; 0xc8uy; 0x99uy; 0x6fuy; 0xb9uy; 0x24uy; *)
-(*       0x27uy; 0xaeuy; 0x41uy; 0xe4uy; 0x64uy; 0x9buy; 0x93uy; 0x4cuy; *)
-(*       0xa4uy; 0x95uy; 0x99uy; 0x1buy; 0x78uy; 0x52uy; 0xb8uy; 0x55uy *)
-(*     ] in *)
+  let expected = FStar.Buffer.createL [
+    0xcfuy; 0x83uy; 0xe1uy; 0x35uy; 0x7euy; 0xefuy; 0xb8uy; 0xbduy;
+    0xf1uy; 0x54uy; 0x28uy; 0x50uy; 0xd6uy; 0x6duy; 0x80uy; 0x07uy;
+    0xd6uy; 0x20uy; 0xe4uy; 0x05uy; 0x0buy; 0x57uy; 0x15uy; 0xdcuy;
+    0x83uy; 0xf4uy; 0xa9uy; 0x21uy; 0xd3uy; 0x6cuy; 0xe9uy; 0xceuy;
+    0x47uy; 0xd0uy; 0xd1uy; 0x3cuy; 0x5duy; 0x85uy; 0xf2uy; 0xb0uy;
+    0xffuy; 0x83uy; 0x18uy; 0xd2uy; 0x87uy; 0x7euy; 0xecuy; 0x2fuy;
+    0x63uy; 0xb9uy; 0x31uy; 0xbduy; 0x47uy; 0x41uy; 0x7auy; 0x81uy;
+    0xa5uy; 0x38uy; 0x32uy; 0x7auy; 0xf9uy; 0x27uy; 0xdauy; 0x3euy
+    ] in
 
-(*   (\* Allocate memory for state *\) *)
-(*   let ctx = FStar.Buffer.create 0uL SHA.hash_size_state_512 in *)
+  (* Allocate memory for state *)
+  let state = FStar.Buffer.create 0uL Hash.size_state in
 
-(*   (\* Call the hash function *\) *)
-(*   SHA.sha2_512 output plaintext plaintext_len; *)
+  (* Call the hash function *)
+  Hash.hash output plaintext plaintext_len;
 
-(*   (\* Display the result *\) *)
-(*   TestLib.compare_and_print (C.string_of_literal "Test 2b") expected output 32ul; *)
+  (* Display the result *)
+  TestLib.compare_and_print (C.string_of_literal "Test 2b") expected output 64ul;
 
-(*   (\* Pop the memory frame *\) *)
-(*   (\**\) pop_frame() *)
+  (* Pop the memory frame *)
+  (**) pop_frame()
 
 
 
@@ -195,12 +203,12 @@ let test_3a () =
   ] in
 
   (* Allocate memory for state *)
-  let ctx = FStar.Buffer.create 0uL SHA.hash_size_state_512 in
+  let state = FStar.Buffer.create 0uL Hash.size_state in
 
   (* Call the hash function *)
-  SHA.sha2_init_512 ctx;
-  SHA.sha2_update_last_512 ctx plaintext plaintext_len;
-  SHA.sha2_finish_512 ctx output;
+  Hash.init state;
+  Hash.update_last state plaintext (FStar.Int.Cast.uint32_to_uint64 plaintext_len);
+  Hash.finish state output;
 
   (* Display the result *)
   TestLib.compare_and_print (C.string_of_literal "Test 3a") expected output 64ul;
@@ -243,10 +251,10 @@ let test_3b () =
   ] in
 
   (* Allocate memory for state *)
-  let ctx = FStar.Buffer.create 0uL SHA.hash_size_state_512 in
+  let state = FStar.Buffer.create 0uL Hash.size_state in
 
   (* Call the hash function *)
-  SHA.sha2_512 output plaintext plaintext_len;
+  Hash.hash output plaintext plaintext_len;
 
   (* Display the result *)
   TestLib.compare_and_print (C.string_of_literal "Test 3b") expected output 64ul;
@@ -297,12 +305,12 @@ let test_4a () =
     ] in
 
   (* Allocate memory for state *)
-  let ctx = FStar.Buffer.create 0uL SHA.hash_size_state_512 in
+  let state = FStar.Buffer.create 0uL Hash.size_state in
 
   (* Call the hash function *)
-  SHA.sha2_init_512 ctx;
-  SHA.sha2_update_last_512 ctx plaintext plaintext_len;
-  SHA.sha2_finish_512 ctx output;
+  Hash.init state;
+  Hash.update_last state plaintext (FStar.Int.Cast.uint32_to_uint64 plaintext_len);
+  Hash.finish state output;
 
   (* Display the result *)
   TestLib.compare_and_print (C.string_of_literal "Test 4a") expected output 64ul;
@@ -352,10 +360,10 @@ let test_4b () =
     ] in
 
   (* Allocate memory for state *)
-  let ctx = FStar.Buffer.create 0uL SHA.hash_size_state_512 in
+  let state = FStar.Buffer.create 0uL Hash.size_state in
 
   (* Call the hash function *)
-  SHA.sha2_512 output plaintext plaintext_len;
+  Hash.hash output plaintext plaintext_len;
 
   (* Display the result *)
   TestLib.compare_and_print (C.string_of_literal "Test 4b") expected output 64ul;
@@ -365,102 +373,119 @@ let test_4b () =
 
 
 
-(* val test_5: unit -> ST unit *)
-(*   (requires (fun h -> True)) *)
-(*   (ensures  (fun h0 r h1 -> True)) *)
-(* let test_5 () = *)
+val test_5: unit -> ST unit
+  (requires (fun h -> True))
+  (ensures  (fun h0 r h1 -> True))
+let test_5 () =
 
-(*   (\* Push a new memory frame *\) *)
-(*   (\**\) push_frame(); *)
+  (* Push a new memory frame *)
+  (**) push_frame();
 
-(*   let output_len = 32ul in *)
-(*   let output = FStar.Buffer.create 0uy output_len in *)
+  let output_len = 64ul in
+  let output = FStar.Buffer.create 0uy output_len in
 
-(*   let plaintext_len = 1000000ul in *)
-(*   let plaintext = FStar.Buffer.create 0x61uy plaintext_len in *)
+  let plaintext_len = 1000000ul in
+  let plaintext = FStar.Buffer.create 0x61uy plaintext_len in
 
-(*   let expected = FStar.Buffer.createL [ *)
-(*       0xcduy; 0xc7uy; 0x6euy; 0x5cuy; 0x99uy; 0x14uy; 0xfbuy; 0x92uy; *)
-(*       0x81uy; 0xa1uy; 0xc7uy; 0xe2uy; 0x84uy; 0xd7uy; 0x3euy; 0x67uy; *)
-(*       0xf1uy; 0x80uy; 0x9auy; 0x48uy; 0xa4uy; 0x97uy; 0x20uy; 0x0euy; *)
-(*       0x04uy; 0x6duy; 0x39uy; 0xccuy; 0xc7uy; 0x11uy; 0x2cuy; 0xd0uy *)
-(*     ] in *)
+  let expected = FStar.Buffer.createL [
+    0xe7uy; 0x18uy; 0x48uy; 0x3duy; 0x0cuy; 0xe7uy; 0x69uy; 0x64uy;
+    0x4euy; 0x2euy; 0x42uy; 0xc7uy; 0xbcuy; 0x15uy; 0xb4uy; 0x63uy;
+    0x8euy; 0x1fuy; 0x98uy; 0xb1uy; 0x3buy; 0x20uy; 0x44uy; 0x28uy;
+    0x56uy; 0x32uy; 0xa8uy; 0x03uy; 0xafuy; 0xa9uy; 0x73uy; 0xebuy;
+    0xdeuy; 0x0fuy; 0xf2uy; 0x44uy; 0x87uy; 0x7euy; 0xa6uy; 0x0auy;
+    0x4cuy; 0xb0uy; 0x43uy; 0x2cuy; 0xe5uy; 0x77uy; 0xc3uy; 0x1buy;
+    0xebuy; 0x00uy; 0x9cuy; 0x5cuy; 0x2cuy; 0x49uy; 0xaauy; 0x2euy;
+    0x4euy; 0xaduy; 0xb2uy; 0x17uy; 0xaduy; 0x8cuy; 0xc0uy; 0x9buy
+    ] in
 
-(*   (\* Allocate memory for state *\) *)
-(*   let ctx = FStar.Buffer.create 0uL SHA.hash_size_state_512 in *)
+  (* Allocate memory for state *)
+  let state = FStar.Buffer.create 0uL Hash.size_state in
 
-(*   (\* Call the hash function *\) *)
-(*   SHA.sha2_512 output plaintext plaintext_len; *)
+  (* Call the hash function *)
+  Hash.hash output plaintext plaintext_len;
 
-(*   (\* Display the result *\) *)
-(*   TestLib.compare_and_print (C.string_of_literal "Test 5") expected output 32ul; *)
+  (* Display the result *)
+  TestLib.compare_and_print (C.string_of_literal "Test 5") expected output 64ul;
 
-(*   (\* Pop the memory frame *\) *)
-(*   (\**\) pop_frame() *)
-
-
-
-(* val test_6_loop: *)
-(*   plaintext:FStar.Buffer.buffer FStar.UInt8.t -> *)
-(*   ctx:FStar.Buffer.buffer FStar.UInt64.t -> *)
-(*   max:FStar.UInt32.t -> *)
-(*   idx:FStar.UInt32.t -> *)
-(*   ST unit *)
-(*   (requires (fun h -> True)) *)
-(*   (ensures  (fun h0 r h1 -> True)) *)
-(* let rec test_6_loop plaintext ctx max idx = *)
-(*   if (idx =^ max) then () *)
-(*   else ( *)
-(*     SHA.sha2_update_512 ctx plaintext; *)
-(*     test_6_loop plaintext ctx max (idx +^ 1ul)) *)
+  (* Pop the memory frame *)
+  (**) pop_frame()
 
 
-(* val test_6: unit -> ST unit *)
-(*   (requires (fun h -> True)) *)
-(*   (ensures  (fun h0 r h1 -> True)) *)
-(* let test_6 () = *)
 
-(*   (\* Push a new memory frame *\) *)
-(*   (\**\) push_frame(); *)
+val test_6_loop:
+  plaintext:FStar.Buffer.buffer FStar.UInt8.t ->
+  state:FStar.Buffer.buffer FStar.UInt64.t ->
+  max:FStar.UInt32.t ->
+  idx:FStar.UInt32.t ->
+  ST unit
+  (requires (fun h -> True))
+  (ensures  (fun h0 r h1 -> True))
+let rec test_6_loop plaintext state max idx =
+  if (idx =^ max) then ()
+  else (
+    Hash.update state plaintext;
+    test_6_loop plaintext state max (idx +^ 1ul))
 
-(*   let output_len = 32ul in *)
-(*   let output = FStar.Buffer.create 0uy output_len in *)
 
-(*   let plaintext_len = 64ul in *)
-(*   let plaintext = FStar.Buffer.createL [ *)
-(*       0x61uy; 0x62uy; 0x63uy; 0x64uy; 0x65uy; 0x66uy; 0x67uy; 0x68uy; *)
-(*       0x62uy; 0x63uy; 0x64uy; 0x65uy; 0x66uy; 0x67uy; 0x68uy; 0x69uy; *)
-(*       0x63uy; 0x64uy; 0x65uy; 0x66uy; 0x67uy; 0x68uy; 0x69uy; 0x6auy; *)
-(*       0x64uy; 0x65uy; 0x66uy; 0x67uy; 0x68uy; 0x69uy; 0x6auy; 0x6buy; *)
-(*       0x65uy; 0x66uy; 0x67uy; 0x68uy; 0x69uy; 0x6auy; 0x6buy; 0x6cuy; *)
-(*       0x66uy; 0x67uy; 0x68uy; 0x69uy; 0x6auy; 0x6buy; 0x6cuy; 0x6duy; *)
-(*       0x67uy; 0x68uy; 0x69uy; 0x6auy; 0x6buy; 0x6cuy; 0x6duy; 0x6euy; *)
-(*       0x68uy; 0x69uy; 0x6auy; 0x6buy; 0x6cuy; 0x6duy; 0x6euy; 0x6fuy *)
-(*   ] in *)
+val test_6: unit -> ST unit
+  (requires (fun h -> True))
+  (ensures  (fun h0 r h1 -> True))
+let test_6 () =
 
-(*   let expected = FStar.Buffer.createL [ *)
-(*       0x50uy; 0xe7uy; 0x2auy; 0x0euy; 0x26uy; 0x44uy; 0x2fuy; 0xe2uy; *)
-(*       0x55uy; 0x2duy; 0xc3uy; 0x93uy; 0x8auy; 0xc5uy; 0x86uy; 0x58uy; *)
-(*       0x22uy; 0x8cuy; 0x0cuy; 0xbfuy; 0xb1uy; 0xd2uy; 0xcauy; 0x87uy; *)
-(*       0x2auy; 0xe4uy; 0x35uy; 0x26uy; 0x6fuy; 0xcduy; 0x05uy; 0x5euy *)
-(*     ] in *)
+  (* Push a new memory frame *)
+  (**) push_frame();
 
-(*   (\* Allocate memory for state *\) *)
-(*   let ctx = FStar.Buffer.create 0uL SHA.hash_size_state_512 in *)
+  let output_len = 64ul in
+  let output = FStar.Buffer.create 0uy output_len in
 
-(*   (\* Sha2_Init_512ialize the hash state *\) *)
-(*   SHA.sha2_init_512 ctx; *)
+  let plaintext_len = 128ul in
+  let plaintext = FStar.Buffer.createL [
+      0x61uy; 0x62uy; 0x63uy; 0x64uy; 0x65uy; 0x66uy; 0x67uy; 0x68uy;
+      0x62uy; 0x63uy; 0x64uy; 0x65uy; 0x66uy; 0x67uy; 0x68uy; 0x69uy;
+      0x63uy; 0x64uy; 0x65uy; 0x66uy; 0x67uy; 0x68uy; 0x69uy; 0x6auy;
+      0x64uy; 0x65uy; 0x66uy; 0x67uy; 0x68uy; 0x69uy; 0x6auy; 0x6buy;
+      0x65uy; 0x66uy; 0x67uy; 0x68uy; 0x69uy; 0x6auy; 0x6buy; 0x6cuy;
+      0x66uy; 0x67uy; 0x68uy; 0x69uy; 0x6auy; 0x6buy; 0x6cuy; 0x6duy;
+      0x67uy; 0x68uy; 0x69uy; 0x6auy; 0x6buy; 0x6cuy; 0x6duy; 0x6euy;
+      0x68uy; 0x69uy; 0x6auy; 0x6buy; 0x6cuy; 0x6duy; 0x6euy; 0x6fuy;
+      0x61uy; 0x62uy; 0x63uy; 0x64uy; 0x65uy; 0x66uy; 0x67uy; 0x68uy;
+      0x62uy; 0x63uy; 0x64uy; 0x65uy; 0x66uy; 0x67uy; 0x68uy; 0x69uy;
+      0x63uy; 0x64uy; 0x65uy; 0x66uy; 0x67uy; 0x68uy; 0x69uy; 0x6auy;
+      0x64uy; 0x65uy; 0x66uy; 0x67uy; 0x68uy; 0x69uy; 0x6auy; 0x6buy;
+      0x65uy; 0x66uy; 0x67uy; 0x68uy; 0x69uy; 0x6auy; 0x6buy; 0x6cuy;
+      0x66uy; 0x67uy; 0x68uy; 0x69uy; 0x6auy; 0x6buy; 0x6cuy; 0x6duy;
+      0x67uy; 0x68uy; 0x69uy; 0x6auy; 0x6buy; 0x6cuy; 0x6duy; 0x6euy;
+      0x68uy; 0x69uy; 0x6auy; 0x6buy; 0x6cuy; 0x6duy; 0x6euy; 0x6fuy
+  ] in
 
-(*   test_6_loop plaintext ctx 16777215ul 0ul; *)
+  let expected = FStar.Buffer.createL [
+    0xb4uy; 0x7cuy; 0x93uy; 0x34uy; 0x21uy; 0xeauy; 0x2duy; 0xb1uy;
+    0x49uy; 0xaduy; 0x6euy; 0x10uy; 0xfcuy; 0xe6uy; 0xc7uy; 0xf9uy;
+    0x3duy; 0x07uy; 0x52uy; 0x38uy; 0x01uy; 0x80uy; 0xffuy; 0xd7uy;
+    0xf4uy; 0x62uy; 0x9auy; 0x71uy; 0x21uy; 0x34uy; 0x83uy; 0x1duy;
+    0x77uy; 0xbeuy; 0x60uy; 0x91uy; 0xb8uy; 0x19uy; 0xeduy; 0x35uy;
+    0x2cuy; 0x29uy; 0x67uy; 0xa2uy; 0xe2uy; 0xd4uy; 0xfauy; 0x50uy;
+    0x50uy; 0x72uy; 0x3cuy; 0x96uy; 0x30uy; 0x69uy; 0x1fuy; 0x1auy;
+    0x05uy; 0xa7uy; 0x28uy; 0x1duy; 0xbeuy; 0x6cuy; 0x10uy; 0x86uy
+    ] in
 
-(*   SHA.sha2_update_last_512 ctx plaintext plaintext_len; *)
-(*   SHA.sha2_finish_512 ctx output; *)
+  (* Allocate memory for state *)
+  let state = FStar.Buffer.create 0uL Hash.size_state in
 
-(*   (\* Display the result *\) *)
-(*   TestLib.compare_and_print (C.string_of_literal "Test 6") expected output 32ul; *)
+  (* initialize the hash state *)
+  Hash.init state;
 
-(*   (\* Pop the memory frame *\) *)
-(*   (\**\) pop_frame() *)
+  test_6_loop plaintext state 8388607ul 0ul;
+
+  let rem_len = UInt32.rem (128ul *%^ 8388607ul) Hash.size_block in
+  Hash.update_last state plaintext (FStar.Int.Cast.uint32_to_uint64 plaintext_len);
+  Hash.finish state output;
+
+  (* Display the result *)
+  TestLib.compare_and_print (C.string_of_literal "Test 6") expected output 64ul;
+
+  (* Pop the memory frame *)
+  (**) pop_frame()
 
 
 
@@ -474,8 +499,8 @@ let main () =
   test_1b ();
 
   (* Run test vector 2 *)
-  (* test_2a (); *)
-  (* test_2b (); *)
+  test_2a ();
+  test_2b ();
 
   (* Run test vector 3 *)
   test_3a ();
@@ -486,10 +511,10 @@ let main () =
   test_4b ();
 
   (* Run test vector 5 *)
-  (* test_5 (); *)
+  test_5 ();
 
   (* Run test vector 6 *)
-  (* test_6(); *)
+  test_6();
 
   (* Exit the program *)
   C.exit_success
